dy-extensions/DY.Simplified.fst
@@ -4,13 +4,34 @@ open Comparse
 open DY.Core
 open DY.Lib
 
-val recv_msg_same_trace:
-  i:timestamp -> tr:trace ->
-  Lemma
-  (ensures (
-    let (opt_msg, tr_out) = recv_msg i tr in
-    tr_out == tr))
-  [SMTPat (recv_msg i tr)
-  ]
-let recv_msg_same_trace i tr =
-  normalize_term_spec recv_msg
+val start_new_session:
+  #a:Type -> {| local_state a |} ->
+  principal -> a ->
+  traceful state_id
+let start_new_session prin cont =
+  let* sid = new_session_id prin in
+  set_state prin sid cont;*
+  return sid
+
+val pk_enc_for:
+  #a:Type -> {| parseable_serializeable bytes a |} ->
+  principal -> principal ->
+  state_id -> string -> 
+  a -> 
+  traceful (option bytes)
+let pk_enc_for #a alice bob key_sid key_tag plaintext =
+  let*? pk_bob = get_public_key alice key_sid (LongTermPkEncKey key_tag) bob in
+  let* nonce = mk_rand PkNonce (principal_label bob) 32 in
+  return ( Some (pk_enc pk_bob nonce (serialize a plaintext)))
+
+val pk_dec_with_key_lookup:
+  #a:Type -> {| parseable_serializeable bytes a |} ->
+  principal -> 
+  state_id -> string ->
+  bytes ->
+  traceful (option a)
+let pk_dec_with_key_lookup #a prin keys_sid key_tag cipher =
+  let*? sk_a = get_private_key prin keys_sid (LongTermPkEncKey key_tag) in
+  let*? plaintext = return (pk_dec sk_a cipher) in 
+  // guard_tr ( Some? (parse a plaintext));*?
+  return (parse a plaintext)
